\documentclass{article}
\usepackage{amsmath}
\usepackage{amssymb}
\usepackage[margin=.5in,left=.5in]{geometry}
\usepackage{amsthm}
\renewcommand{\qedsymbol}{QED}

\begin{document}

\noindent The triple integral of a function \( f(x, y, z) \) over a box \( B \) is written as:
\[
\iiint_B f(x, y, z) \, dV.
\]

\begin{proof}

\noindent For simplicity, we can start with a simple double integral. This principle can be applied to any arbitrary n-number of iterated integrals.
\[
\iint_Rf(x,y) \, dA.
\]

\noindent For any iterated integral of some function $f(x,y)$ in any Euclidean coordinate system (e.g. Cartesian, polar, and cylindrical), such that $f(x,y)$ can be expressed as the product of two independent functions $g(x)$ and $h(y)$, and that the bounds of integration are constants:

\[
\int_{c}^{d} \int_{a}^{b} f(x, y) \, dA = \int_{c}^{d} \int_{a}^{b} g(x)h(y) \,dxdy
\]

\[
\{(a, b, c, d) \in \mathbb{R}\}
\]

\[
h(y) \text{ is a constant when you integrate with respect to } x.
\]

\[
g(x) \text{ is a constant when you integrate with respect to } y.
\]

\noindent We can represent this as the product of two definite integrals of functions that are independent of each other:

\[
\int_{a}^{b}g(x) \,dx \cdot \int_{c}^{d}h(y) \,dy
\]

\noindent If this claim is true, it must also apply to partial derivatives due to the Fundamental Theorem of Calculus.\\

\noindent Suppose some function $f(x, y) = x^2 y^3$.

\[
f(x, y) = g(x) \cdot h(y); \quad g(x) = x^2, \quad h(y) = y^3
\]

\[
\frac{\partial^{2} f}{\partial x \partial y} = \frac{\partial^{2}f}{\partial y \partial x} = 6xy^{2}
\]

\[\frac{\partial g}{\partial x} = 2x\]
\[\frac{\partial h}{\partial y} = 3y^{2}\]
\[\frac{\partial g}{\partial x} \cdot \frac{\partial h}{\partial y} = 6xy^{2}\]
Thus:

\[
\frac{\partial^2 f}{\partial x \partial y} = \frac{\partial^2 f}{\partial y \partial x} = \frac{\partial g}{\partial x} \cdot \frac{\partial h}{\partial y} = \frac{dg}{dx} \cdot \frac{dh}{dy}
\]

\noindent Therefore, if and only if $f_i(x_i)$ is independent from $f_{i+1}(x_{i+1})$
\[
\prod_{i=1}^n \int_{a_i}^{b_i} f_i(x_i) \, dx_i = \int_{a_1}^{b_1} f_1(x_1) \, dx_1 \cdot \int_{a_2}^{b_2} f_2(x_2) \, dx_2 \cdots \int_{a_n}^{b_n} f_n(x_n) \, dx_n
\]

\[
\{(a_i, b_i) \in \mathbb{R}\mid i \in \mathbb{N} \}
\]

\noindent The proof is trivial.

\end{proof}

\end{document}